src/example.v
@@ -3,8 +3,6 @@ From TLA Require Import defs automation logic.
 (* TODO: move to library *)
 #[global] Hint Unfold state_pred action_pred : tla.
 
-(* TODO: rename `next` to something else (maybe prime) *)
-
 Section lib.
 
 Context [Σ: Type].
@@ -24,7 +22,7 @@ Qed.
 
 Lemma action_preserves_inv (p: Σ → Prop) (a: action Σ) :
     (∀ s s', p s → a s s' → p s') →
-    state_pred p ∧ ⟨a⟩ ⊢ next (state_pred p).
+    state_pred p ∧ ⟨a⟩ ⊢ later (state_pred p).
 Proof.
   intros H.
   unseal.
@@ -41,18 +39,18 @@ Hint Rewrite drop_n : tla.
 
 Hint Unfold leads_to : tla.
 
-Lemma wf1 (p q: predicate) (Next a: Σ → Σ → Prop) :
-  (⊢ p ∧ ⟨Next⟩ → next p ∨ next q) →
-  (⊢ p ∧ ⟨Next⟩ ∧ ⟨a⟩ → next q) →
+Lemma wf1 (p q: predicate) (next a: Σ → Σ → Prop) :
+  (⊢ p ∧ ⟨next⟩ → later p ∨ later q) →
+  (⊢ p ∧ ⟨next⟩ ∧ ⟨a⟩ → later q) →
   (⊢ p → enabled a) →
-  (⊢ □ ⟨Next⟩ ∧ weak_fairness a → leads_to p q).
+  (⊢ □ ⟨next⟩ ∧ weak_fairness a → leads_to p q).
 Proof.
   intros H1 H2 H3.
   rewrite weak_fairness_alt1'.
   autounfold with tla in *.
   setoid_rewrite drop_n.
   simpl.
-  intros e [Hnext Hwf].
+  intros e [Hlater Hwf].
   intros k Hp.
   setoid_rewrite drop_drop.
   rewrite /weak_fairness in Hwf; autounfold with tla in Hwf.
@@ -84,13 +82,13 @@ Definition ab : action state :=
 Definition bc : action state :=
   λ s s', (s.(x) = B ∧ s'.(x) = C ∧ s'.(happy) = s.(happy)).
 
-Definition Next s s' :=
+Definition next s s' :=
   ab s s' ∨ bc s s' ∨ s = s'.
 
 Definition init (s: state) : Prop := s.(x) = A ∧ s.(happy).
 
 Theorem always_happy :
-  state_pred init ∧ □ ⟨Next⟩ ⊢ □ (state_pred (λ s, s.(happy))).
+  state_pred init ∧ □ ⟨next⟩ ⊢ □ (state_pred (λ s, s.(happy))).
 Proof.
   apply (init_safety _ _ (state_pred (λ s, s.(happy))) _).
   - apply state_pred_impl.
@@ -100,7 +98,7 @@ Proof.
   - apply action_preserves_inv => s s'.
 
     (* SM reasoning *)
-    rewrite /happy /Next /ab /bc.
+    rewrite /happy /next /ab /bc.
     destruct s, s'; simpl.
     intuition (subst; auto).
     congruence.
@@ -108,7 +106,7 @@ Proof.
 Qed.
 
 Theorem a_leads_to_b :
-  □ ⟨ Next ⟩ ∧ weak_fairness ab ⊢
+  □ ⟨ next ⟩ ∧ weak_fairness ab ⊢
   leads_to (state_pred (λ s, s.(x) = A)) (state_pred (λ s, s.(x) = B)).
 Proof.
   apply wf1.
@@ -117,7 +115,7 @@ Proof.
     generalize dependent (e 1); intros s'.
     clear e.
     intuition auto.
-    rewrite /Next in H1.
+    rewrite /next in H1.
     rewrite /ab /bc in H1.
     intuition (eauto; try congruence).
   - unseal; rewrite /drop /=.
@@ -140,7 +138,7 @@ Proof.
 Qed.
 
 Theorem eventually_b :
-  state_pred init ∧ □ ⟨Next⟩ ∧ weak_fairness ab ⊢
+  state_pred init ∧ □ ⟨next⟩ ∧ weak_fairness ab ⊢
   ◇ (state_pred (λ s, s.(x) = B)).
 Proof.
   rewrite -> a_leads_to_b.
@@ -152,19 +150,19 @@ Proof.
 Qed.
 
 Theorem b_leads_to_c :
-  □ ⟨ Next ⟩ ∧ weak_fairness bc ⊢
+  □ ⟨ next ⟩ ∧ weak_fairness bc ⊢
   leads_to (state_pred (λ s, s.(x) = B)) (state_pred (λ s, s.(x) = C)).
 Proof.
 Admitted.
 
 Theorem a_leads_to_c :
-  □ ⟨ Next ⟩ ∧ weak_fairness ab ∧ weak_fairness bc ⊢
+  □ ⟨ next ⟩ ∧ weak_fairness ab ∧ weak_fairness bc ⊢
   leads_to (state_pred (λ s, s.(x) = A)) (state_pred (λ s, s.(x) = C)).
 Proof.
 Admitted.
 
 Theorem eventually_c :
-  state_pred init ∧ □ ⟨Next⟩ ∧ weak_fairness ab ∧ weak_fairness bc ⊢
+  state_pred init ∧ □ ⟨next⟩ ∧ weak_fairness ab ∧ weak_fairness bc ⊢
   ◇ (state_pred (λ s, s.(x) = C)).
 Proof.
 Admitted.
